Monad_Play Around/DNFP/Dutch_National_Flag_Monad.thy
@@ -5,7 +5,7 @@ imports
 begin
 
 section\<open>DNFP\<close>
-text\<open>A version using a state monad for storing the array and the intermediate variable.
+text\<open>A version using a state-monad for storing the array and the intermediate variable.
 This function takes a parameter that defines the size of the unsorted array (the difference between high and i).
 This makes the recursion well-defined and will ensure termination since loop-update-action decreases the difference for every single call\<close>
 fun dnfp_mon:: "nat \<Rightarrow> (env, unit) state" where
@@ -19,91 +19,84 @@ fun dnfp_mon:: "nat \<Rightarrow> (env, unit) state" where
                        else skip
                       )}"
 
-subsection\<open>DNFP preserves the Invariants proof\<close>
+subsection\<open>DNFP - Invariants proof\<close>
 lemma dnfp_invariantRed: "spec (dnfp_inv1) (dnfp_mon n) (GG dnfp_inv1)"
   unfolding dnfp_inv1_def GG_def 
   apply(induction n rule: dnfp_mon.induct)
-    apply(simp add: spec_def)
-    apply(simp add: skip_def)
+  apply(simp add: spec_def skip_def)
   apply(simp only: caseN)
-   apply(intro get_rule; intro allI; clarify)
+  apply(intro get_rule; intro allI; clarify)
   apply(intro cond_rule; simp)
-   apply(simp add: loop_update_action_def)
-   apply(intro get_rule; intro allI; clarify)
+  apply(simp add: loop_update_action_def)
+  apply(intro get_rule; intro allI; clarify)
   apply(intro seq_rule[of _ _ "(\<lambda>x e. dnfp_variables_invariants e \<and> low_invariant_is_0_Env e)"])
-    apply(intro cond_rule)
-  apply (smt GG_def One_nat_def case_prodD case_prodI2 inc_lowbound_inv1_aux_def inc_lowbound_inv1_def inc_lowbound_invariantRed lessI loop_update_action_pre_def prod.simps(1) spec_def)
-  apply (smt GG_def case_prodD case_prodI2 dec_highbound_inv1_aux_def dec_highbound_inv1_def dec_highbound_invariantRed loop_update_action_pre_def prod.simps(1) spec_def)
-    apply (smt GG_def case_prodD case_prodI2 inc_index_inv1_aux_def inc_index_inv1_def inc_index_invariantRed less_one loop_update_action_pre_def prod.simps(1) spec_def) 
-   apply blast
-    apply(simp add: spec_def)
-   by(simp add: skip_def)
+  apply(intro cond_rule)
+  apply (smt GG_def Pair_inject dnfp_inv1_def inc_lowbound_inv1_def inc_lowbound_invariantRed less_numeral_extra(1) loop_update_action_inv1_def loop_update_action_pre_def spec_def split_beta')
+  apply (smt GG_def Pair_inject dec_highbound_inv1_def dec_highbound_invariantRed dnfp_inv1_def loop_update_action_inv1_def loop_update_action_pre_def spec_def split_beta')
+  apply (smt GG_def Pair_inject dnfp_inv1_def inc_index_inv1_def inc_index_invariantRed less_one loop_update_action_inv1_def loop_update_action_pre_def spec_def split_beta')
+  apply blast
+  by(simp add: spec_def skip_def)
 
 lemma dnfp_invariantWhite: "spec dnfp_inv2 (dnfp_mon n) (GG dnfp_inv2)"
   unfolding dnfp_inv2_def  GG_def
   apply(induction n rule: dnfp_mon.induct)
-    apply(simp add: spec_def)
-    apply(simp add: skip_def)
+  apply(simp add: spec_def skip_def)
   apply(simp only: caseN)
-   apply(intro get_rule; intro allI; clarify)
+  apply(intro get_rule; intro allI; clarify)
   apply(intro cond_rule; simp)
   apply(simp add: loop_update_action_def)
-   apply(intro get_rule; intro allI; clarify)
+  apply(intro get_rule; intro allI; clarify)
   apply(intro seq_rule[of _ _ "(\<lambda>x e. dnfp_variables_invariants e \<and> invariant_low_to_j_is_1_Env e)"])
-    apply(intro cond_rule; simp)
-      apply (smt GG_def One_nat_def case_prodD case_prodI2 inc_lowbound_inv2_aux_def inc_lowbound_inv2_def inc_lowbound_invariantWhite lessI loop_update_action_pre_def spec_def)
-     apply (smt GG_def One_nat_def case_prodD case_prodI2 dec_highbound_inv2_aux_def dec_highbound_inv2_def dec_highbound_invariantWhite loop_update_action_pre_def spec_def)
-  apply (smt GG_def One_nat_def Suc_less_eq inc_index_inv2_aux_def inc_index_inv2_def inc_index_invariantWhite less_Suc_eq loop_update_action_pre_def spec_def split_beta')
+  apply(intro cond_rule; simp)
+  apply (smt GG_def dnfp_inv2_def inc_lowbound_inv2_def inc_lowbound_invariantWhite less_numeral_extra(1) loop_update_action_inv2_def loop_update_action_pre_def spec_def split_beta')
+  apply (smt GG_def One_nat_def dec_highbound_inv2_def dec_highbound_invariantWhite dnfp_inv2_def loop_update_action_inv2_def loop_update_action_pre_def spec_def split_beta')
+  apply (smt GG_def One_nat_def dnfp_inv2_def inc_index_inv2_def inc_index_invariantWhite loop_update_action_inv2_def loop_update_action_pre_def not_less_eq spec_def split_beta')
   apply blast
-    apply(simp add: spec_def)
-   by(simp add: skip_def)
+  by(simp add: spec_def skip_def)
 
 lemma dnfp_invariantBlue: "spec dnfp_inv3 (dnfp_mon n) (GG dnfp_inv3)"
   unfolding dnfp_inv3_def GG_def
   apply(induction n rule: dnfp_mon.induct)
-    apply(simp add: spec_def)
-    apply(simp add: skip_def)
+  apply(simp add: spec_def skip_def)
   apply(simp only: caseN)
-   apply(intro get_rule; intro allI; clarify)
+  apply(intro get_rule; intro allI; clarify)
   apply(intro cond_rule; simp)
   apply(simp add: loop_update_action_def)
-   apply(intro get_rule; intro allI; clarify)
+  apply(intro get_rule; intro allI; clarify)
   apply(intro seq_rule[of _ _ "(\<lambda>x e. dnfp_variables_invariants e \<and> high_invariant_is_2_Env e)"])
-    apply (intro cond_rule; simp)
-      apply (smt GG_def One_nat_def case_prodD case_prodI2 inc_lowbound_inv3_aux_def inc_lowbound_inv3_def inc_lowbound_invariantBlue lessI loop_update_action_pre_def spec_def)
-     apply (smt GG_def One_nat_def dec_highbound_inv3_aux_def dec_highbound_inv3_def dec_highbound_invariantBlue loop_update_action_pre_def spec_def split_beta')
-  apply (smt GG_def One_nat_def Suc_less_eq inc_index_inv3_aux_def inc_index_inv3_def inc_index_invariantBlue less_Suc_eq loop_update_action_pre_def spec_def split_beta')
- apply blast
-     apply(simp add: spec_def)
-  by(simp add: skip_def)
+  apply (intro cond_rule; simp)
+  apply (smt GG_def dnfp_inv3_def inc_lowbound_inv3_def inc_lowbound_invariantBlue less_numeral_extra(1) loop_update_action_inv3_def loop_update_action_pre_def spec_def split_beta')
+  apply (smt GG_def One_nat_def dec_highbound_inv3_def dec_highbound_invariantBlue dnfp_inv3_def loop_update_action_inv3_def loop_update_action_pre_def spec_def split_beta')
+  apply (smt GG_def One_nat_def dnfp_inv3_def inc_index_inv3_def inc_index_invariantBlue loop_update_action_inv3_def loop_update_action_pre_def not_less_eq spec_def split_beta')
+  apply blast
+  by(simp add: spec_def skip_def)
 
-text\<open>All invariants are preserved by the function\<close>
-lemma dnfp_mon_invariants: "spec (dnfp_mon_inv) (dnfp_mon n) (GG dnfp_mon_inv)"
-  by (smt GG_def dnfp_invariantBlue dnfp_invariantRed dnfp_invariantWhite dnfp_mon_inv_def spec_def split_def)
+text\<open>All invariants are preserved by the dnfp-function\<close>
+lemma dnfp_mon_invariants: "spec (dnfp_inv) (dnfp_mon n) (GG dnfp_inv)"
+  by (smt GG_def dnfp_invariantBlue dnfp_invariantRed dnfp_invariantWhite dnfp_inv_def spec_def split_def)
 
 section\<open>Main proof\<close>
 
-text\<open>If the invariants are kept and i = high, when the entire array will be sorted\<close>
+text\<open>The invariants and i = high means that the the entire array will be sorted\<close>
 lemma dnfp_mon_isSorted: "dnfp_post_final_spec e \<Longrightarrow> sorted (xs e)" 
-  unfolding dnfp_post_final_spec_def dnfp_mon_inv_def
+  unfolding dnfp_post_final_spec_def dnfp_inv_def
   by (smt Suc_1 Suc_leD dnfp_inv1_def dnfp_inv2_def dnfp_inv3_def high_invariant_is_2_Env_def invariant_low_to_j_is_1_Env_def less_numeral_extra(1) less_or_eq_imp_le less_trans low_invariant_is_0_Env_def not_less sorted_iff_nth_mono_less)
 
 text\<open>DNFP mon preserves the invariants on the ranges and the bounds of the variables\<close>
 lemma dnfp_mon_main: "spec (dnfp_mon_spec) (dnfp_mon n) (GG dnfp_mon_spec)"
   unfolding GG_def dnfp_mon_spec_def
   apply(induction n rule: dnfp_mon.induct)
-    apply(simp add: spec_def)
-   apply(simp add: skip_def)
+  apply(simp add: spec_def skip_def)
   apply(simp only: caseN)
   apply(intro get_rule; intro allI; clarify)
   apply(intro cond_rule)
-   apply(simp add: loop_update_action_def)
-   apply(intro get_rule; intro allI; clarify)
-   apply(intro seq_rule[of _ _ "(\<lambda>x e. dnfp_variables_invariants e \<and> dnfp_mon_inv e)"])
-    apply(intro cond_rule)
-      apply (smt GG_def Pair_inject dnfp_inv1_def dnfp_inv2_def dnfp_inv3_def dnfp_mon_inv_def inc_lowbound_inv1_aux_def inc_lowbound_inv1_def inc_lowbound_inv2_aux_def inc_lowbound_inv2_def inc_lowbound_inv3_aux_def inc_lowbound_inv3_def inc_lowbound_invariantBlue inc_lowbound_invariantRed inc_lowbound_invariantWhite less_numeral_extra(1) loop_update_action_pre_def spec_def split_beta')
-  apply (smt GG_def Pair_inject dec_highbound_inv1_aux_def dec_highbound_inv1_def dec_highbound_inv2_aux_def dec_highbound_inv2_def dec_highbound_inv3_aux_def dec_highbound_inv3_def dec_highbound_invariantBlue dec_highbound_invariantRed dec_highbound_invariantWhite dnfp_inv1_def dnfp_inv2_def dnfp_inv3_def dnfp_mon_inv_def loop_update_action_pre_def spec_def split_beta')
-  apply (smt GG_def Pair_inject dnfp_inv1_def dnfp_inv2_def dnfp_inv3_def dnfp_mon_inv_def inc_index_inv1_aux_def inc_index_inv1_def inc_index_inv2_aux_def inc_index_inv2_def inc_index_inv3_aux_def inc_index_inv3_def inc_index_invariantBlue inc_index_invariantRed inc_index_invariantWhite less_one loop_update_action_pre_def spec_def split_beta') 
+  apply(simp add: loop_update_action_def)
+  apply(intro get_rule; intro allI; clarify)
+  apply(intro seq_rule[of _ _ "(\<lambda>x e. dnfp_variables_invariants e \<and> dnfp_inv e)"])
+  apply(intro cond_rule)
+  apply (smt GG_def Pair_inject dnfp_inv1_def dnfp_inv_def inc_lowbound_inv1_def inc_lowbound_inv2_def inc_lowbound_inv3_def inc_lowbound_invariantBlue inc_lowbound_invariantRed inc_lowbound_invariantWhite less_numeral_extra(1) loop_update_action_inv1_def loop_update_action_inv2_def loop_update_action_inv3_def loop_update_action_pre_def spec_def split_beta')
+  apply (smt GG_def Pair_inject dec_highbound_inv1_def dec_highbound_inv2_def dec_highbound_inv3_def dec_highbound_invariantBlue dec_highbound_invariantRed dec_highbound_invariantWhite dnfp_inv1_def dnfp_inv_def loop_update_action_inv1_def loop_update_action_inv2_def loop_update_action_inv3_def loop_update_action_pre_def spec_def split_beta')
+  apply (smt GG_def Pair_inject dnfp_inv1_def dnfp_inv_def inc_index_inv1_def inc_index_inv2_def inc_index_inv3_def inc_index_invariantBlue inc_index_invariantRed inc_index_invariantWhite less_one loop_update_action_inv1_def loop_update_action_inv2_def loop_update_action_inv3_def loop_update_action_pre_def spec_def split_beta')
   apply blast
   by(simp add: spec_def skip_def)
 
@@ -117,32 +110,32 @@ lemma aux1: "(spec (\<lambda>e. dnfp_variables_invariants e \<and> n = high e - 
             (loop_update_action \<bind> (\<lambda>_. dnfp_mon n)) (\<lambda>x e. high e = i e)"
   apply(intro seq_rule[of _ _ "(\<lambda>x e. dnfp_variables_invariants e
                                 \<and> n = high e - i e)"])
-   apply(simp add: loop_update_action_def)
-   apply(intro get_rule; intro allI; clarify)
-   apply(intro cond_rule)
-     apply(simp add: inc_lowbound_def)
-     apply(intro get_rule; intro allI; simp)
+  apply(simp add: loop_update_action_def)
+  apply(intro get_rule; intro allI; clarify)
+  apply(intro cond_rule)
+  apply(simp add: inc_lowbound_def)
+  apply(intro get_rule; intro allI; simp)
   apply(intro seq_rule[of _ _ "(\<lambda>x e. Suc n = high e - i e \<and> high e > i e \<and> dnfp_variables_invariants e)"])
-      apply(simp add: spec_def swap_def xs_Env_def put_def get_state_def put_state_def dnfp_variables_invariants_def)
-   apply(intro allI; simp)
-      apply(intro get_rule; intro allI)
+  apply(simp add: spec_def swap_def xs_Env_def put_def get_state_def put_state_def dnfp_variables_invariants_def)
+  apply(intro allI; simp)
+  apply(intro get_rule; intro allI)
   apply(intro seq_rule[of _ _ "(\<lambda>x e. n = high e - i e \<and> dnfp_variables_invariants e \<and> i e > low e)"])
   apply(simp add: spec_def i_Env_def put_def get_state_def put_state_def dnfp_variables_invariants_def)
   apply linarith
-   apply(intro allI; simp)
-      apply(intro get_rule; intro allI; simp)
-       apply(simp add: spec_def low_Env_def put_def get_state_def put_state_def dnfp_variables_invariants_def)
-     apply(simp add: dec_highbound_def)
-     apply(intro get_rule; intro allI; simp)
+  apply(intro allI; simp)
+  apply(intro get_rule; intro allI; simp)
+  apply(simp add: spec_def low_Env_def put_def get_state_def put_state_def dnfp_variables_invariants_def)
+  apply(simp add: dec_highbound_def)
+  apply(intro get_rule; intro allI; simp)
   apply(intro seq_rule[of _ _ "(\<lambda>x e. n = high e - i e \<and> dnfp_variables_invariants e)"])
-     apply(simp add: spec_def high_Env_def put_def get_state_def put_state_def dnfp_variables_invariants_def)
+  apply(simp add: spec_def high_Env_def put_def get_state_def put_state_def dnfp_variables_invariants_def)
   apply linarith
-   apply(intro allI; simp)
-      apply(intro get_rule; intro allI; simp)
-        apply(simp add: spec_def swap_def xs_Env_def put_def get_state_def put_state_def dnfp_variables_invariants_def)
-        apply(simp add: inc_index_def)
-      apply(intro get_rule; intro allI; simp)
-   apply(simp add: spec_def i_Env_def put_def get_state_def put_state_def dnfp_variables_invariants_def)
+  apply(intro allI; simp)
+  apply(intro get_rule; intro allI; simp)
+  apply(simp add: spec_def swap_def xs_Env_def put_def get_state_def put_state_def dnfp_variables_invariants_def)
+  apply(simp add: inc_index_def)
+  apply(intro get_rule; intro allI; simp)
+  apply(simp add: spec_def i_Env_def put_def get_state_def put_state_def dnfp_variables_invariants_def)
   apply linarith
   by blast
 
@@ -153,11 +146,9 @@ This can be used the termination. And this proof can together with the dnfp-mon 
 lemma dnfp_mon_termination: "spec (dnfp_mon_pre n) (dnfp_mon n) (GG (i_high_equal n))"
   unfolding GG_def dnfp_mon_pre_def dnfp_mon_spec_def i_high_equal_def
   apply(induction n rule: dnfp_mon.induct)
-    apply(simp add: spec_def)
-   apply(simp add: skip_def)
-  apply (simp add: dnfp_variables_invariants_def)
+  apply(simp add: spec_def skip_def dnfp_variables_invariants_def)
   apply(simp only: caseN)
-   apply(intro get_rule; intro allI; clarify)
+  apply(intro get_rule; intro allI; clarify)
   apply(intro cond_rule)
   using aux1 apply blast
   by(simp add: spec_def skip_def dnfp_variables_invariants_def)
@@ -174,6 +165,7 @@ definition init_env:: "nat array \<Rightarrow> env" where
   "init_env l \<equiv> \<lparr>high = (length l),            low = 0,
                  i = 0,                         xs = l\<rparr>"
 
+text\<open>A proof to show that the init-env will satisfy the invariant of the environment\<close>
 lemma "e = (init_env x) \<and> set(x) \<subseteq> {0,1,2} \<Longrightarrow> dnfp_variables_invariants e"
   unfolding init_env_def dnfp_variables_invariants_def
   by simp
