Monad_Play Around/DNFP/Dutch_National_Flag_Monad_Definitions_Lemmas.thy
@@ -3,8 +3,9 @@ imports
   "Dutch_National_Flag_Monad_Eisbach"
 begin
 
-section\<open>Aux lemmas about values inside the array\<close>
+section\<open>Aux. lemmas about values inside the array\<close>
 
+text\<open>These proofs have been made to make Isabelle able to inferer the correct value at position i in the array\<close>
 lemma value_must_be_one : "\<lbrakk>xs e ! i e  \<noteq> 0 ; xs e! i e \<noteq> 2 ; i e < length (xs e) ; set(xs e) \<subseteq> {0,1,2}\<rbrakk> \<Longrightarrow> xs e ! i e = 1"
   by (smt insertE insert_subset mk_disjoint_insert nth_mem singletonD)
 
@@ -21,106 +22,105 @@ lemma value_must_be_one_aux : "\<lbrakk>\<not>xs e ! i e  > 1 ; \<not>xs e! i e 
   by linarith
 
 section\<open>Inc lowbound - proof\<close>
-
-text\<open>Inc lowbound will keep relationship between variables and inc i and low\<close>
+text\<open>Inc lowbound will keep the relationship between variables and both the i and low variable will be increased\<close>
 lemma inc_lowbound_spec: "spec (inc_lowbound_pre e) inc_lowbound (GG (inc_lowbound_post e))"
   unfolding inc_lowbound_pre_def loop_update_action_pre_def dnfp_variables_invariants_def GG_def inc_lowbound_post_def loop_update_action_post_def dnfp_post_def
   apply(simp_all add: inc_lowbound_def)
   apply(intro get_rule; intro allI; simp)
   apply(intro conj_rule_right)
-           apply(intro seq_rule[of _ _ "(\<lambda>_ y. high e = high y)"])
+  apply(intro seq_rule[of _ _ "(\<lambda>_ y. high e = high y)"])
   apply(rewrite_env simps: swap_def xs_Env_def)
   apply(intro allI; simp)
-         apply(intro get_rule; intro allI)
-           apply (intro seq_rule[of _ _ "(\<lambda>_ y. high e = high y)"])
+  apply(intro get_rule; intro allI)
+  apply (intro seq_rule[of _ _ "(\<lambda>_ y. high e = high y)"])
   apply(rewrite_env simps: i_Env_def)
   apply(rewrite_env simps: low_Env_def)
-          apply (intro seq_rule[of _ _ "(\<lambda>_ y. low e = low y)"])
-  apply(rewrite_env_all)
+  apply (intro seq_rule[of _ _ "(\<lambda>_ y. low e = low y)"])
+  apply(rewrite_env simps: xs_Env_def swap_def)
   apply(all_Get_Seq)
-        apply(intro seq_rule[of _ _ "(\<lambda>_ y. low e = low y)"])
-          apply (simp add: spec_def put_def put_state_def swap_def get_state_def i_Env_def)
-          apply(all_Get_Seq)
-
-        apply(simp add: spec_def put_def get_state_def put_state_def low_Env_def)
-       apply (intro seq_rule[of _ _ "(\<lambda>_ y. length (xs e) = length (xs y))"])
-        apply (simp add: spec_def put_def put_state_def swap_def get_state_def xs_Env_def i_Env_def)
-         apply(all_Get_Seq)
-         apply (intro seq_rule[of _ _ "(\<lambda>_ y. length (xs e) = length (xs y))"])
-        apply (simp add: spec_def put_def put_state_def swap_def get_state_def i_Env_def)
-       apply(intro allI; simp)
-       apply(intro get_rule; intro allI)
-       apply(simp add: spec_def put_def get_state_def put_state_def low_Env_def)
-      apply (intro seq_rule[of _ _ "(\<lambda>_ y. high y = high e)"])
-       apply (simp add: spec_def put_def put_state_def swap_def get_state_def xs_Env_def i_Env_def)
-       apply(intro allI; simp)
-       apply(intro get_rule; intro allI)
+  apply(intro seq_rule[of _ _ "(\<lambda>_ y. low e = low y)"])
+  apply (simp add: spec_def put_def put_state_def swap_def get_state_def i_Env_def)
+  apply(all_Get_Seq)
+  apply(simp add: spec_def put_def get_state_def put_state_def low_Env_def)
+  apply (intro seq_rule[of _ _ "(\<lambda>_ y. length (xs e) = length (xs y))"])
+  apply (simp add: spec_def put_def put_state_def swap_def get_state_def xs_Env_def i_Env_def)
+  apply(all_Get_Seq)
+  apply (intro seq_rule[of _ _ "(\<lambda>_ y. length (xs e) = length (xs y))"])
+  apply (simp add: spec_def put_def put_state_def swap_def get_state_def i_Env_def)
+  apply(intro allI; simp)
+  apply(intro get_rule; intro allI)
+  apply(simp add: spec_def put_def get_state_def put_state_def low_Env_def)
   apply (intro seq_rule[of _ _ "(\<lambda>_ y. high y = high e)"])
-       apply (simp add: spec_def put_def put_state_def swap_def get_state_def i_Env_def)
-      apply(intro allI; simp)
-      apply(intro get_rule; intro allI)
-      apply(simp add: spec_def put_def get_state_def put_state_def low_Env_def)
-     apply (intro seq_rule[of _ _ "(\<lambda>_ y. low y = low e)"])
-      apply (simp add: spec_def put_def put_state_def swap_def get_state_def xs_Env_def i_Env_def)
-     apply(intro allI; simp)
-     apply(intro get_rule; intro allI)
-     apply (intro seq_rule[of _ _ "(\<lambda>_ y. low y = low e)"])
-      apply (simp add: spec_def put_def put_state_def swap_def get_state_def i_Env_def)
-     apply(intro allI; simp)
-     apply(intro get_rule; intro allI)
-     apply(simp add: spec_def put_def get_state_def put_state_def low_Env_def)
-     apply (intro seq_rule[of _ _ "(\<lambda>_ y. i y = i e)"])
-     apply (simp add: spec_def put_def put_state_def swap_def get_state_def xs_Env_def i_Env_def)
-    apply(intro allI; simp)
-    apply(intro get_rule; intro allI)
-     apply (intro seq_rule[of _ _ "(\<lambda>_ y. i y > i e)"])
-     apply (simp add: spec_def put_def put_state_def swap_def get_state_def i_Env_def)
-    apply(intro allI; simp)
-    apply(intro get_rule; intro allI)
-    apply(simp add: spec_def put_def get_state_def put_state_def low_Env_def)
-   apply (intro seq_rule[of _ _ "(\<lambda>_ y. high y - i y \<le> high e - i e)"])
-     apply (simp add: spec_def put_def put_state_def swap_def get_state_def xs_Env_def i_Env_def)
-   apply(intro allI; simp)
-   apply(intro get_rule; intro allI)
-   apply (intro seq_rule[of _ _ "(\<lambda>_ y. high y - i y \<le> high e - i e)"])
-    apply (simp add: spec_def put_def put_state_def swap_def get_state_def i_Env_def)
-    apply (linarith)
-   apply(intro allI; simp)
-   apply(intro get_rule; intro allI)
-    apply(simp add: spec_def put_def get_state_def put_state_def low_Env_def)
-   apply (intro seq_rule[of _ _ "(\<lambda>x y. mset (xs e) = mset (xs y))"])
-   apply (simp add: spec_def put_def put_state_def swap_def get_state_def xs_Env_def i_Env_def)
+  apply (simp add: spec_def put_def put_state_def swap_def get_state_def xs_Env_def i_Env_def)
+  apply(intro allI; simp)
+  apply(intro get_rule; intro allI)
+  apply (intro seq_rule[of _ _ "(\<lambda>_ y. high y = high e)"])
+  apply (simp add: spec_def put_def put_state_def swap_def get_state_def i_Env_def)
+  apply(intro allI; simp)
+  apply(intro get_rule; intro allI)
+  apply(simp add: spec_def put_def get_state_def put_state_def low_Env_def)
+  apply (intro seq_rule[of _ _ "(\<lambda>_ y. low y = low e)"])
+  apply (simp add: spec_def put_def put_state_def swap_def get_state_def xs_Env_def i_Env_def)
+  apply(intro allI; simp)
+  apply(intro get_rule; intro allI)
+  apply (intro seq_rule[of _ _ "(\<lambda>_ y. low y = low e)"])
+  apply (simp add: spec_def put_def put_state_def swap_def get_state_def i_Env_def)
+  apply(intro allI; simp)
+  apply(intro get_rule; intro allI)
+  apply(simp add: spec_def put_def get_state_def put_state_def low_Env_def)
+  apply (intro seq_rule[of _ _ "(\<lambda>_ y. i y = i e)"])
+  apply (simp add: spec_def put_def put_state_def swap_def get_state_def xs_Env_def i_Env_def)
+  apply(intro allI; simp)
+  apply(intro get_rule; intro allI)
+  apply (intro seq_rule[of _ _ "(\<lambda>_ y. i y > i e)"])
+  apply (simp add: spec_def put_def put_state_def swap_def get_state_def i_Env_def)
+  apply(intro allI; simp)
+  apply(intro get_rule; intro allI)
+  apply(simp add: spec_def put_def get_state_def put_state_def low_Env_def)
+  apply (intro seq_rule[of _ _ "(\<lambda>_ y. high y - i y \<le> high e - i e)"])
+  apply (simp add: spec_def put_def put_state_def swap_def get_state_def xs_Env_def i_Env_def)
+  apply(intro allI; simp)
+  apply(intro get_rule; intro allI)
+  apply (intro seq_rule[of _ _ "(\<lambda>_ y. high y - i y \<le> high e - i e)"])
+  apply (simp add: spec_def put_def put_state_def swap_def get_state_def i_Env_def)
+  apply (linarith)
+  apply(intro allI; simp)
+  apply(intro get_rule; intro allI)
+  apply(simp add: spec_def put_def get_state_def put_state_def low_Env_def)
+  apply (intro seq_rule[of _ _ "(\<lambda>x y. mset (xs e) = mset (xs y))"])
+  apply (simp add: spec_def put_def put_state_def swap_def get_state_def xs_Env_def i_Env_def)
   apply (metis (no_types, hide_lams) Multiset.mset_swap le_less_trans less_le_trans)
-    apply(intro allI; simp)
-   apply(intro get_rule; intro allI)
-   apply (intro seq_rule[of _ _ "(\<lambda>x y. mset (xs e) = mset (xs y))"])
-   apply (simp add: spec_def put_def put_state_def swap_def get_state_def i_Env_def)
-   apply(intro allI; simp)
-   apply(intro get_rule; intro allI)
-   apply(simp add: spec_def put_def get_state_def put_state_def low_Env_def)
-   apply (intro seq_rule[of _ _ "(\<lambda>x y. high y - i y = high e - i e \<and> high e > i e)"])
-    apply (simp add: spec_def put_def put_state_def swap_def get_state_def xs_Env_def)
-   apply(intro allI; simp)
-   apply(intro get_rule; intro allI)
-   apply (intro seq_rule[of _ _ "(\<lambda>x y. Suc(high y - i y) = high e - i e)"])
-    apply (simp add: spec_def put_def put_state_def get_state_def i_Env_def)
+  apply(intro allI; simp)
+  apply(intro get_rule; intro allI)
+  apply (intro seq_rule[of _ _ "(\<lambda>x y. mset (xs e) = mset (xs y))"])
+  apply (simp add: spec_def put_def put_state_def swap_def get_state_def i_Env_def)
+  apply(intro allI; simp)
+  apply(intro get_rule; intro allI)
+  apply(simp add: spec_def put_def get_state_def put_state_def low_Env_def)
+  apply (intro seq_rule[of _ _ "(\<lambda>x y. high y - i y = high e - i e \<and> high e > i e)"])
+  apply (simp add: spec_def put_def put_state_def swap_def get_state_def xs_Env_def)
+  apply(intro allI; simp)
+  apply(intro get_rule; intro allI)
+  apply (intro seq_rule[of _ _ "(\<lambda>x y. Suc(high y - i y) = high e - i e)"])
+  apply (simp add: spec_def put_def put_state_def get_state_def i_Env_def)
   apply linarith
-   apply(intro allI; simp)
-   apply(intro get_rule; intro allI)
-   apply(simp add: spec_def put_def get_state_def put_state_def low_Env_def)
-   apply (intro seq_rule[of _ _ "(\<lambda>x y. i y \<ge> i e)"])
-    apply (simp add: spec_def put_def put_state_def swap_def get_state_def xs_Env_def)
-   apply(intro allI; simp)
-   apply(intro get_rule; intro allI)
-   apply (intro seq_rule[of _ _ "(\<lambda>x y. i y > i e)"])
-    apply (simp add: spec_def put_def put_state_def get_state_def i_Env_def)
-   apply(intro allI; simp)
-   apply(intro get_rule; intro allI)
+  apply(intro allI; simp)
+  apply(intro get_rule; intro allI)
+  apply(simp add: spec_def put_def get_state_def put_state_def low_Env_def)
+  apply (intro seq_rule[of _ _ "(\<lambda>x y. i y \<ge> i e)"])
+  apply (simp add: spec_def put_def put_state_def swap_def get_state_def xs_Env_def)
+  apply(intro allI; simp)
+  apply(intro get_rule; intro allI)
+  apply (intro seq_rule[of _ _ "(\<lambda>x y. i y > i e)"])
+  apply (simp add: spec_def put_def put_state_def get_state_def i_Env_def)
+  apply(intro allI; simp)
+  apply(intro get_rule; intro allI)
   by(simp add: spec_def put_def get_state_def put_state_def low_Env_def)
 
 subsection\<open>Invariants - inc lowbound\<close>
-lemma inc_lowbound_invariantRed: "spec inc_lowbound_inv1_aux inc_lowbound (GG inc_lowbound_inv1)"
-  unfolding inc_lowbound_inv1_aux_def inc_lowbound_inv1_def loop_update_action_pre_def  GG_def low_invariant_is_0_Env_def dnfp_variables_invariants_def
+text\<open>These proofs show that the invariants on the ranges are kept by a inc lowbound action\<close>
+lemma inc_lowbound_invariantRed: "spec inc_lowbound_inv1 inc_lowbound (GG dnfp_inv1)"
+  unfolding inc_lowbound_inv1_def loop_update_action_pre_def  GG_def loop_update_action_inv1_def dnfp_inv1_def low_invariant_is_0_Env_def dnfp_variables_invariants_def
   apply(simp_all add: inc_lowbound_def)
   apply(intro get_rule; intro allI; simp)
   apply(intro seq_rule[of _ _ "(\<lambda>x s. i s < high s \<and>
@@ -128,7 +128,7 @@ lemma inc_lowbound_invariantRed: "spec inc_lowbound_inv1_aux inc_lowbound (GG in
                  high s \<le> length (xs s) \<and>
                  set (xs s) \<subseteq> {0, 1, 2} \<and>
                  (\<forall>x \<le> low s. xs s ! x = 0))"])
-   apply (simp add: spec_def put_def put_state_def swap_def get_state_def xs_Env_def)
+  apply (simp add: spec_def put_def put_state_def swap_def get_state_def xs_Env_def)
   apply (smt length_list_update less_le_trans nth_list_update order.not_eq_order_implies_strict set_swap)
   apply(intro allI; simp)
   apply(intro get_rule; intro allI)
@@ -137,13 +137,13 @@ lemma inc_lowbound_invariantRed: "spec inc_lowbound_inv1_aux inc_lowbound (GG in
                  high s \<le> length (xs s) \<and>
                  set (xs s) \<subseteq> {0, 1, 2} \<and>
                  (\<forall>x\<le>low s. xs s ! x = 0))"])
-   apply (simp add: spec_def put_def put_state_def get_state_def i_Env_def)
+  apply (simp add: spec_def put_def put_state_def get_state_def i_Env_def)
   apply(intro allI; simp)
   apply(intro get_rule; intro allI)
   by (simp add: spec_def put_def put_state_def get_state_def low_Env_def)
 
-lemma inc_lowbound_invariantWhite: "spec inc_lowbound_inv2_aux inc_lowbound (GG inc_lowbound_inv2)"
-  unfolding inc_lowbound_inv2_aux_def inc_lowbound_inv2_def loop_update_action_pre_def  GG_def invariant_low_to_j_is_1_Env_def dnfp_variables_invariants_def
+lemma inc_lowbound_invariantWhite: "spec inc_lowbound_inv2 inc_lowbound (GG dnfp_inv2)"
+  unfolding inc_lowbound_inv2_def loop_update_action_inv2_def  inc_lowbound_inv2_def loop_update_action_pre_def dnfp_inv2_def GG_def invariant_low_to_j_is_1_Env_def dnfp_variables_invariants_def
   apply(simp_all add: inc_lowbound_def)
   apply(intro get_rule; intro allI; simp)
   apply(intro seq_rule[of _ _ "(\<lambda>x s. i s < high s \<and>
@@ -151,22 +151,22 @@ lemma inc_lowbound_invariantWhite: "spec inc_lowbound_inv2_aux inc_lowbound (GG 
                  high s \<le> length (xs s) \<and>
                  set (xs s) \<subseteq> {0, 1, 2} \<and>
                  (\<forall>x. low s < x \<and> x \<le> i s \<longrightarrow> xs s ! x = 1))"])
-   apply (simp add: spec_def put_def put_state_def get_state_def xs_Env_def swap_def)
+  apply (simp add: spec_def put_def put_state_def get_state_def xs_Env_def swap_def)
   apply (smt le_less less_le_trans nth_list_update set_swap)
-   apply(intro allI; simp)
+  apply(intro allI; simp)
   apply(intro get_rule; intro allI)
   apply(intro seq_rule[of _ _ "(\<lambda>x s. i s \<le> high s \<and>
                  low s < i s \<and>
                  high s \<le> length (xs s) \<and>
                  set (xs s) \<subseteq> {0, 1, 2} \<and>
                  (\<forall>x. low s < x \<and> x < i s \<longrightarrow> xs s ! x = 1))"])
-   apply (simp add: spec_def put_def put_state_def  get_state_def i_Env_def)
-   apply(intro allI; simp)
+  apply (simp add: spec_def put_def put_state_def  get_state_def i_Env_def)
+  apply(intro allI; simp)
   apply(intro get_rule; intro allI)
   by (simp add: spec_def put_def put_state_def  get_state_def low_Env_def)
 
-lemma inc_lowbound_invariantBlue: "spec inc_lowbound_inv3_aux  inc_lowbound (GG inc_lowbound_inv3)"
-  unfolding inc_lowbound_inv3_aux_def inc_lowbound_inv3_def loop_update_action_pre_def  GG_def high_invariant_is_2_Env_def dnfp_variables_invariants_def
+lemma inc_lowbound_invariantBlue: "spec inc_lowbound_inv3  inc_lowbound (GG dnfp_inv3)"
+  unfolding  inc_lowbound_inv3_def loop_update_action_inv3_def loop_update_action_pre_def dnfp_inv3_def  GG_def high_invariant_is_2_Env_def dnfp_variables_invariants_def
   apply(simp_all add: inc_lowbound_def)
   apply(intro get_rule; intro allI; simp)
   apply(intro seq_rule[of _ _ "(\<lambda>x s. 
@@ -175,23 +175,24 @@ lemma inc_lowbound_invariantBlue: "spec inc_lowbound_inv3_aux  inc_lowbound (GG 
                        set (xs s) \<subseteq> {0, 1, 2} \<and>
                        i s < high s \<and>
                        (\<forall>x. high s \<le> x \<and> x < length (xs s) \<longrightarrow> xs s ! x = 2))"])
-   apply (simp add: spec_def put_def put_state_def swap_def get_state_def xs_Env_def)
+  apply (simp add: spec_def put_def put_state_def swap_def get_state_def xs_Env_def)
   apply (smt less_le_trans not_less set_swap)
-   apply(intro allI; simp)
+  apply(intro allI; simp)
   apply(intro get_rule; intro allI)
   apply(intro seq_rule[of _ _ "(\<lambda>x s. i s \<le> high s \<and>
                  low s < i s \<and>
                  high s \<le> length (xs s) \<and>
                  set (xs s) \<subseteq> {0, 1, 2} \<and>
                  (\<forall>x. high s \<le> x \<and> x < length (xs s) \<longrightarrow> xs s ! x = 2))"])
-   apply (simp add: spec_def put_def put_state_def get_state_def i_Env_def)
+  apply (simp add: spec_def put_def put_state_def get_state_def i_Env_def)
   apply(intro allI; simp)
   apply(intro get_rule; intro allI)
   by (simp add: spec_def put_def put_state_def get_state_def low_Env_def)
 
 text\<open>All invariants are preserved\<close>
-lemma inc_lowbound_invariants: "spec inc_lowbound_inv_pre  inc_lowbound (GG inc_lowbound_inv)"
-  by (smt GG_def case_prodD case_prodI2 inc_lowbound_inv1_aux_def inc_lowbound_inv2_aux_def inc_lowbound_inv3_aux_def inc_lowbound_inv_def inc_lowbound_inv_pre_def inc_lowbound_invariantBlue inc_lowbound_invariantRed inc_lowbound_invariantWhite spec_def)
+lemma inc_lowbound_invariants: "spec inc_lowbound_inv_pre  inc_lowbound (GG dnfp_inv)"
+  unfolding inc_lowbound_inv_pre_def GG_def dnfp_inv_def loop_update_action_inv_def
+  by (smt GG_def inc_lowbound_inv1_def inc_lowbound_inv2_def inc_lowbound_inv3_def inc_lowbound_invariantBlue inc_lowbound_invariantRed inc_lowbound_invariantWhite loop_update_action_inv1_def loop_update_action_inv2_def loop_update_action_inv3_def spec_def split_beta')
 
 section\<open>Dec highbound proof\<close>                                          
 lemma dec_highbound_spec: "spec (dec_highbound_pre e) dec_highbound (GG (dec_highbound_post e))"
@@ -199,119 +200,121 @@ lemma dec_highbound_spec: "spec (dec_highbound_pre e) dec_highbound (GG (dec_hig
   apply(simp_all add: dec_highbound_def)
   apply(intro get_rule; intro allI; simp)
   apply(intro conj_rule_right)
-   apply(intro seq_rule[of _ _ "(\<lambda>_ y. high y < length (xs y))"])
-       apply (simp add: spec_def put_def put_state_def get_state_def high_Env_def)
+  apply(intro seq_rule[of _ _ "(\<lambda>_ y. high y < length (xs y))"])
+  apply (simp add: spec_def put_def put_state_def get_state_def high_Env_def)
   apply linarith
-           apply(intro allI; simp)
-           apply(intro get_rule; intro allI; simp)
-             apply (simp add: spec_def put_def put_state_def get_state_def xs_Env_def swap_def)
-             apply(intro seq_rule[of _ _ "(\<lambda>_ y. high y < high e)"])
-             apply (simp add: spec_def put_def put_state_def get_state_def high_Env_def)
-           apply(intro allI; simp)
-            apply(intro get_rule; intro allI; simp)
-             apply (simp add: spec_def put_def put_state_def get_state_def xs_Env_def)
-          apply(intro seq_rule[of _ _ "(\<lambda>_ y. low e = low y)"])
-           apply (simp add: spec_def put_def put_state_def get_state_def high_Env_def)
-           apply(intro allI; simp)
-          apply(intro get_rule; intro allI; simp)
-             apply (simp add: spec_def put_def put_state_def get_state_def xs_Env_def)
-        apply(intro seq_rule[of _ _ "(\<lambda>_ y. i e = i y)"])
-            apply (simp add: spec_def put_def put_state_def get_state_def high_Env_def)
-           apply(intro allI; simp)
-          apply(intro get_rule; intro allI; simp)
-          apply (simp add: spec_def put_def put_state_def get_state_def xs_Env_def)
-        apply(intro seq_rule[of _ _ "(\<lambda>_ y. xs y ! i y = 2 \<and> high y < length(xs y) \<and> high y \<ge> i y)"])
-          apply (simp add: spec_def put_def put_state_def get_state_def high_Env_def)
-        using less_le_trans value_must_be_two_aux1 apply auto[1]
-           apply(intro allI; simp)
-          apply(intro get_rule; intro allI; simp)
-       apply (simp add: spec_def put_def put_state_def get_state_def xs_Env_def swap_def)
-          apply(intro seq_rule[of _ _ "(\<lambda>_ y. length (xs e) = length (xs y))"])
-      apply (simp add: spec_def put_def put_state_def get_state_def high_Env_def)
-       apply(intro allI; simp)
-       apply(intro get_rule; intro allI; simp)
-       apply (simp add: spec_def put_def put_state_def get_state_def xs_Env_def swap_def)
-      apply(intro seq_rule[of _ _ "(\<lambda>_ y. high y \<le> high e)"])
-          apply (simp add: spec_def put_def put_state_def get_state_def high_Env_def)
-         apply(intro allI; simp)
-      apply(intro get_rule; intro allI; simp)
-      apply (simp add: spec_def put_def put_state_def get_state_def xs_Env_def)
-     apply(intro seq_rule[of _ _ "(\<lambda>_ y. low e \<le> low y)"])
-      apply (simp add: spec_def put_def put_state_def get_state_def high_Env_def)
-       apply(intro allI; simp)
-      apply(intro get_rule; intro allI; simp)
-      apply (simp add: spec_def put_def put_state_def get_state_def xs_Env_def)
-     apply(intro seq_rule[of _ _ "(\<lambda>_ y. i e \<le> i y)"])
-      apply (simp add: spec_def put_def put_state_def get_state_def high_Env_def)
-       apply(intro allI; simp)
-      apply(intro get_rule; intro allI; simp)
-      apply (simp add: spec_def put_def put_state_def get_state_def xs_Env_def)
-     apply(intro seq_rule[of _ _ "(\<lambda>_ y. high y - i y \<le> high e - i e)"])
-       apply (simp add: spec_def put_def put_state_def get_state_def high_Env_def)
+  apply(intro allI; simp)
+  apply(intro get_rule; intro allI; simp)
+  apply (simp add: spec_def put_def put_state_def get_state_def xs_Env_def swap_def)
+  apply(intro seq_rule[of _ _ "(\<lambda>_ y. high y < high e)"])
+  apply (simp add: spec_def put_def put_state_def get_state_def high_Env_def)
+  apply(intro allI; simp)
+  apply(intro get_rule; intro allI; simp)
+  apply (simp add: spec_def put_def put_state_def get_state_def xs_Env_def)
+  apply(intro seq_rule[of _ _ "(\<lambda>_ y. low e = low y)"])
+  apply (simp add: spec_def put_def put_state_def get_state_def high_Env_def)
+  apply(intro allI; simp)
+  apply(intro get_rule; intro allI; simp)
+  apply (simp add: spec_def put_def put_state_def get_state_def xs_Env_def)
+  apply(intro seq_rule[of _ _ "(\<lambda>_ y. i e = i y)"])
+  apply (simp add: spec_def put_def put_state_def get_state_def high_Env_def)
+  apply(intro allI; simp)
+  apply(intro get_rule; intro allI; simp)
+  apply (simp add: spec_def put_def put_state_def get_state_def xs_Env_def)
+  apply(intro seq_rule[of _ _ "(\<lambda>_ y. xs y ! i y = 2 \<and> high y < length(xs y) \<and> high y \<ge> i y)"])
+  apply (simp add: spec_def put_def put_state_def get_state_def high_Env_def)
+  using less_le_trans value_must_be_two_aux1 apply auto[1]
+  apply(intro allI; simp)
+  apply(intro get_rule; intro allI; simp)
+  apply (simp add: spec_def put_def put_state_def get_state_def xs_Env_def swap_def)
+  apply(intro seq_rule[of _ _ "(\<lambda>_ y. length (xs e) = length (xs y))"])
+  apply (simp add: spec_def put_def put_state_def get_state_def high_Env_def)
+  apply(intro allI; simp)
+  apply(intro get_rule; intro allI; simp)
+  apply (simp add: spec_def put_def put_state_def get_state_def xs_Env_def swap_def)
+  apply(intro seq_rule[of _ _ "(\<lambda>_ y. high y \<le> high e)"])
+  apply (simp add: spec_def put_def put_state_def get_state_def high_Env_def)
+  apply(intro allI; simp)
+  apply(intro get_rule; intro allI; simp)
+  apply (simp add: spec_def put_def put_state_def get_state_def xs_Env_def)
+  apply(intro seq_rule[of _ _ "(\<lambda>_ y. low e \<le> low y)"])
+  apply (simp add: spec_def put_def put_state_def get_state_def high_Env_def)
+  apply(intro allI; simp)
+  apply(intro get_rule; intro allI; simp)
+  apply (simp add: spec_def put_def put_state_def get_state_def xs_Env_def)
+  apply(intro seq_rule[of _ _ "(\<lambda>_ y. i e \<le> i y)"])
+  apply (simp add: spec_def put_def put_state_def get_state_def high_Env_def)
+  apply(intro allI; simp)
+  apply(intro get_rule; intro allI; simp)
+  apply (simp add: spec_def put_def put_state_def get_state_def xs_Env_def)
+  apply(intro seq_rule[of _ _ "(\<lambda>_ y. high y - i y \<le> high e - i e)"])
+  apply (simp add: spec_def put_def put_state_def get_state_def high_Env_def)
   apply (simp add: diff_le_mono2)
-       apply(intro allI; simp)
-   apply(intro get_rule; intro allI; simp)
-      apply (simp add: spec_def put_def put_state_def get_state_def xs_Env_def)
-     apply(intro seq_rule[of _ _ "(\<lambda>_ y. mset (xs e) = mset (xs y))"])
-       apply (simp add: spec_def put_def put_state_def get_state_def high_Env_def)
-     apply(intro allI; simp)
-     apply(intro get_rule; intro allI; simp)
-         apply (simp add: spec_def put_def put_state_def get_state_def swap_def xs_Env_def)
-        apply (simp add: mset_swap)
-   apply (intro seq_rule[of _ _ "(\<lambda>x y. Suc(high y - i y) = high e - i e \<and> high e > i e)"])
-         apply (simp add: spec_def put_def put_state_def get_state_def high_Env_def)
-        apply linarith
-   apply(intro allI; simp)
-   apply(intro get_rule; intro allI; simp)
-        by (simp add: spec_def put_def put_state_def get_state_def xs_Env_def)
+  apply(intro allI; simp)
+  apply(intro get_rule; intro allI; simp)
+  apply (simp add: spec_def put_def put_state_def get_state_def xs_Env_def)
+  apply(intro seq_rule[of _ _ "(\<lambda>_ y. mset (xs e) = mset (xs y))"])
+  apply (simp add: spec_def put_def put_state_def get_state_def high_Env_def)
+  apply(intro allI; simp)
+  apply(intro get_rule; intro allI; simp)
+  apply (simp add: spec_def put_def put_state_def get_state_def swap_def xs_Env_def)
+  apply (simp add: mset_swap)
+  apply (intro seq_rule[of _ _ "(\<lambda>x y. Suc(high y - i y) = high e - i e \<and> high e > i e)"])
+  apply (simp add: spec_def put_def put_state_def get_state_def high_Env_def)
+  apply linarith
+  apply(intro allI; simp)
+  apply(intro get_rule; intro allI; simp)
+  by (simp add: spec_def put_def put_state_def get_state_def xs_Env_def)
   
 subsection\<open>Invariants - dec highbound\<close>
-lemma dec_highbound_invariantRed: "spec dec_highbound_inv1_aux dec_highbound (GG dec_highbound_inv1)"
-    unfolding dec_highbound_inv1_aux_def dec_highbound_inv1_def dnfp_variables_invariants_def loop_update_action_pre_def GG_def low_invariant_is_0_Env_def
+text\<open>These proofs show that the invariants on the ranges are kept by a dec highbound action\<close>
+lemma dec_highbound_invariantRed: "spec dec_highbound_inv1 dec_highbound (GG dnfp_inv1)"
+    unfolding dec_highbound_inv1_def dec_highbound_inv1_def loop_update_action_inv1_def dnfp_inv1_def dnfp_variables_invariants_def loop_update_action_pre_def GG_def low_invariant_is_0_Env_def
     apply(simp_all add: dec_highbound_def)
     apply(intro get_rule; intro allI; simp)
     apply(intro seq_rule[of _ _ "(\<lambda>x e. i e \<le> high e \<and>
                  low e \<le> i e \<and>
                  high e \<le> length (xs e) \<and>
                  set (xs e) \<subseteq> {0, 1, 2} \<and> Suc 0 < xs e ! i e \<and> (\<forall>x < low e. xs e ! x = 0))"])
-     apply (simp add: spec_def put_def put_state_def get_state_def high_Env_def swap_def)
+    apply (simp add: spec_def put_def put_state_def get_state_def high_Env_def swap_def)
     apply linarith
-     apply(intro allI; simp)
+    apply(intro allI; simp)
     apply(intro get_rule;intro allI; simp)
     by (simp add: spec_def put_def put_state_def get_state_def xs_Env_def swap_def)
 
 
-lemma dec_highbound_invariantWhite: "spec dec_highbound_inv2_aux dec_highbound (GG dec_highbound_inv2)"
-    unfolding dec_highbound_inv2_aux_def dec_highbound_inv2_def dnfp_variables_invariants_def loop_update_action_pre_def GG_def invariant_low_to_j_is_1_Env_def
+lemma dec_highbound_invariantWhite: "spec dec_highbound_inv2 dec_highbound (GG dnfp_inv2)"
+    unfolding dec_highbound_inv2_def dec_highbound_inv2_def loop_update_action_inv2_def dnfp_inv2_def  dnfp_variables_invariants_def loop_update_action_pre_def GG_def invariant_low_to_j_is_1_Env_def
     apply(simp_all add: dec_highbound_def)
-        apply(intro get_rule; intro allI; simp)
+    apply(intro get_rule; intro allI; simp)
     apply(intro seq_rule[of _ _ "(\<lambda>x e. i e \<le> high e \<and>
                  low e \<le> i e \<and>
                  high e \<le> length (xs e) \<and>
                  set (xs e) \<subseteq> {0, 1, 2} \<and> Suc 0 < xs e ! i e \<and> (\<forall>x. low e \<le> x \<and> x < i e \<longrightarrow> xs e ! x = Suc 0))"])
-     apply (simp add: spec_def put_def put_state_def get_state_def high_Env_def swap_def)
+    apply (simp add: spec_def put_def put_state_def get_state_def high_Env_def swap_def)
     apply linarith
-     apply(intro allI; simp)
+    apply(intro allI; simp)
     apply(intro get_rule;intro allI; simp)
     by (simp add: spec_def put_def put_state_def get_state_def xs_Env_def swap_def)
 
-lemma dec_highbound_invariantBlue: "spec dec_highbound_inv3_aux dec_highbound (GG dec_highbound_inv3)"
-    unfolding dec_highbound_inv3_aux_def dec_highbound_inv3_def dnfp_variables_invariants_def loop_update_action_pre_def GG_def high_invariant_is_2_Env_def
+lemma dec_highbound_invariantBlue: "spec dec_highbound_inv3 dec_highbound (GG dnfp_inv3)"
+    unfolding dec_highbound_inv3_def dec_highbound_inv3_def loop_update_action_inv3_def dnfp_inv3_def dnfp_variables_invariants_def loop_update_action_pre_def GG_def high_invariant_is_2_Env_def
     apply(simp_all add: dec_highbound_def)
     apply(intro get_rule; intro allI; simp)
-   apply(intro seq_rule[of _ _ "(\<lambda>x e. i e \<le> high e \<and>
+    apply(intro seq_rule[of _ _ "(\<lambda>x e. i e \<le> high e \<and>
                  low e \<le> i e \<and>
                  high e \<le> length (xs e) \<and>
                  set (xs e) \<subseteq> {0, 1, 2} \<and> Suc 0 < xs e ! i e \<and> (\<forall>x. high e < x \<and> x < length (xs e) \<longrightarrow> xs e ! x = 2))"])
-     apply (simp add: spec_def put_def put_state_def get_state_def high_Env_def swap_def)
-     apply force
-     apply(intro allI; simp)
+    apply (simp add: spec_def put_def put_state_def get_state_def high_Env_def swap_def)
+    apply force
+    apply(intro allI; simp)
     apply(intro get_rule;intro allI; simp)
     apply (simp add: spec_def put_def put_state_def get_state_def xs_Env_def swap_def)
     by (smt One_nat_def leD le_eq_less_or_eq le_less_trans length_list_update less_numeral_extra(2) nth_list_update value_must_be_two_aux)
 
-lemma dec_highbound_invariants: "spec dec_highbound_inv_aux dec_highbound (GG dec_highbound_inv)"
-  by (smt GG_def case_prodD case_prodI2 dec_highbound_inv1_aux_def dec_highbound_inv2_aux_def dec_highbound_inv3_aux_def dec_highbound_inv_aux_def dec_highbound_inv_def dec_highbound_invariantBlue dec_highbound_invariantRed dec_highbound_invariantWhite spec_def)
+lemma dec_highbound_invariants: "spec dec_highbound_inv dec_highbound (GG dnfp_inv)"
+  unfolding dec_highbound_inv_def loop_update_action_inv_def GG_def dnfp_inv_def
+  by (smt GG_def case_prodD dec_highbound_inv1_def dec_highbound_inv2_def dec_highbound_inv3_def dec_highbound_invariantBlue dec_highbound_invariantRed dec_highbound_invariantWhite loop_update_action_inv1_def loop_update_action_inv2_def loop_update_action_inv3_def spec_def split_cong)
 
 section\<open>Inc index proof\<close>
 lemma inc_index_spec: "spec (inc_index_pre e) inc_index (GG (inc_index_post e))"
@@ -320,218 +323,221 @@ lemma inc_index_spec: "spec (inc_index_pre e) inc_index (GG (inc_index_post e))"
   apply(intro get_rule; intro allI;simp)
   apply(intro conj_rule_right)
   apply (simp_all add: spec_def put_def put_state_def get_state_def i_Env_def)
-   apply linarith
+  apply linarith
   by linarith
 
 subsection\<open>Invariants - inc index\<close>
-lemma inc_index_invariantRed: "spec inc_index_inv1_aux inc_index (GG inc_index_inv1)"
-  unfolding inc_index_inv1_aux_def inc_index_inv1_def dnfp_variables_invariants_def loop_update_action_pre_def  GG_def low_invariant_is_0_Env_def
+text\<open>These proofs show that the invariants on the ranges are kept by a inc index action. It can be noted that these proofs are very simple do the fact that the definition only contains one put-statement. 
+And nothing follows the put-statement. It is therefore not necessary to introduce the seq-rule.)\<close>
+lemma inc_index_invariantRed: "spec inc_index_inv1 inc_index (GG dnfp_inv1)"
+  unfolding inc_index_inv1_def loop_update_action_inv1_def dnfp_variables_invariants_def dnfp_inv1_def loop_update_action_pre_def  GG_def low_invariant_is_0_Env_def
   apply(simp_all add: inc_index_def)
   apply(intro get_rule; intro allI; simp)
   by (simp add: spec_def i_Env_def put_def get_state_def put_state_def)
                                
-lemma inc_index_invariantWhite: "spec inc_index_inv2_aux inc_index (GG inc_index_inv2)"
-  unfolding inc_index_inv2_aux_def dnfp_variables_invariants_def inc_index_inv2_def loop_update_action_pre_def  GG_def invariant_low_to_j_is_1_Env_def
+lemma inc_index_invariantWhite: "spec inc_index_inv2 inc_index (GG dnfp_inv2)"
+  unfolding inc_index_inv2_def loop_update_action_inv2_def dnfp_variables_invariants_def dnfp_inv2_def loop_update_action_pre_def  GG_def invariant_low_to_j_is_1_Env_def
   apply(simp_all add: inc_index_def)
   apply(intro get_rule; intro allI; simp)
   apply (simp add: spec_def i_Env_def put_def get_state_def put_state_def)
   using le_eq_less_or_eq by fastforce
 
-lemma inc_index_invariantBlue: "spec inc_index_inv3_aux inc_index (GG inc_index_inv3)"
-  unfolding inc_index_inv3_aux_def inc_index_inv3_def dnfp_variables_invariants_def loop_update_action_pre_def  GG_def high_invariant_is_2_Env_def
+lemma inc_index_invariantBlue: "spec inc_index_inv3 inc_index (GG dnfp_inv3)"
+  unfolding inc_index_inv3_def loop_update_action_inv3_def  dnfp_variables_invariants_def dnfp_inv3_def loop_update_action_pre_def  GG_def high_invariant_is_2_Env_def
   apply(simp_all add: inc_index_def)
   apply(intro get_rule; intro allI; simp)
   by (simp add: spec_def i_Env_def put_def get_state_def put_state_def)
 
-lemma inc_index_invariants: "spec inc_index_inv_aux inc_index (GG inc_index_inv)"
-  unfolding inc_index_inv_aux_def inc_index_inv_def GG_def
-  by (smt GG_def case_prod_beta' inc_index_inv1_aux_def inc_index_inv2_aux_def inc_index_inv3_aux_def inc_index_invariantBlue inc_index_invariantRed inc_index_invariantWhite spec_def)
+lemma inc_index_invariants: "spec inc_index_inv inc_index (GG dnfp_inv)"
+  unfolding inc_index_inv_def dnfp_inv_def GG_def loop_update_action_inv_def
+  by (smt GG_def inc_index_inv1_def inc_index_inv2_def inc_index_inv3_def inc_index_invariantBlue inc_index_invariantRed inc_index_invariantWhite loop_update_action_inv1_def loop_update_action_inv2_def loop_update_action_inv3_def spec_def split_beta')
 
 section\<open>Loop update action - proofs\<close>
+text\<open>This proofs shows that the loop-update-action preserves the relationship on the variables. This proof can be rewritten to make use of the lemmas established in the file above.\<close>
 lemma loop_update_action_spec: "spec (loop_update_action_pre_aux e) loop_update_action (GG (loop_update_action_post e))"
   unfolding loop_update_action_pre_aux_def GG_def loop_update_action_post_def loop_update_action_pre_def dnfp_variables_invariants_def dnfp_post_def
   apply(simp add: loop_update_action_def)
   apply (intro get_rule; intro allI; clarify)
   apply (intro cond_rule)
-    apply(simp add: inc_lowbound_def)
- apply(intro get_rule; intro allI; simp)
-    apply(intro conj_rule_right)
-       apply (intro seq_rule[of _ _ "(\<lambda>_ y. length (xs e) = length (xs y))"])
-          apply (simp add: spec_def put_def put_state_def swap_def get_state_def xs_Env_def)
-        apply(intro allI; simp)
-        apply(intro get_rule; intro allI)
-       apply (intro seq_rule[of _ _ "(\<lambda>_ y. length (xs e) = length (xs y))"])
-          apply (simp add: spec_def put_def put_state_def swap_def get_state_def i_Env_def)
-         apply(intro allI; simp)
-        apply(intro get_rule; intro allI)
-          apply (simp add: spec_def put_def put_state_def swap_def get_state_def low_Env_def)
-         apply (intro seq_rule[of _ _ "(\<lambda>_ y. high e = high y)"])
-        apply (simp add: spec_def put_def put_state_def swap_def get_state_def xs_Env_def)
-         apply(intro allI; simp)
-        apply(intro get_rule; intro allI)
-         apply (intro seq_rule[of _ _ "(\<lambda>_ y. high e = high y)"])
-          apply (simp add: spec_def put_def put_state_def swap_def get_state_def i_Env_def)
-         apply(intro allI; simp)
-       apply(intro get_rule; intro allI)
-          apply (simp add: spec_def put_def put_state_def swap_def get_state_def low_Env_def)
-      apply (intro seq_rule[of _ _ "(\<lambda>_ y. low e = low y)"])
-          apply (simp add: spec_def put_def put_state_def swap_def get_state_def xs_Env_def i_Env_def)
-        apply(intro allI; simp)
-        apply(intro get_rule; intro allI)
-        apply(intro seq_rule[of _ _ "(\<lambda>_ y. low e = low y)"])
-          apply (simp add: spec_def put_def put_state_def  get_state_def i_Env_def)
-        apply(intro allI; simp)
-        apply(intro get_rule; intro allI)
-      apply(simp add: spec_def put_def get_state_def put_state_def low_Env_def)
-     apply (intro seq_rule[of _ _ "(\<lambda>_ y. i y = i e)"])
-     apply (simp add: spec_def put_def put_state_def swap_def get_state_def xs_Env_def)
-    apply(intro allI; simp)
-    apply(intro get_rule; intro allI)
-     apply (intro seq_rule[of _ _ "(\<lambda>_ y. i y > i e)"])
-      apply (simp add: spec_def put_def put_state_def  get_state_def i_Env_def)
-    apply(intro allI; simp)
-     apply(intro get_rule; intro allI)
-      apply (simp add: spec_def put_def put_state_def  get_state_def low_Env_def)
-   apply (intro seq_rule[of _ _ "(\<lambda>_ y. i y < high y \<and> i y = i e \<and> high y = high e)"])
-    apply (simp add: spec_def put_def put_state_def swap_def get_state_def xs_Env_def)
-   apply(intro allI; simp)
-   apply(intro get_rule; intro allI)
-   apply (intro seq_rule[of _ _ "(\<lambda>_ y. high y - i y < high e - i e)"])
-    apply (simp add: spec_def put_def put_state_def  get_state_def i_Env_def)
-     apply (linarith)
-   apply(intro allI; simp)
-   apply(intro get_rule; intro allI)
-     apply (simp add: spec_def put_def put_state_def  get_state_def low_Env_def)
-   apply (intro seq_rule[of _ _ "(\<lambda>_ y. mset(xs e) = mset(xs y))"])
-    apply (simp add: spec_def put_def put_state_def swap_def get_state_def xs_Env_def)
-     apply (simp add: Multiset.mset_swap)
-   apply(intro allI; simp)
-    apply(intro get_rule; intro allI)
-   apply (intro seq_rule[of _ _ "(\<lambda>_ y. mset(xs e) = mset(xs y))"])
-     apply (simp add: spec_def put_def put_state_def get_state_def i_Env_def)
-   apply(intro allI; simp)
-    apply(intro get_rule; intro allI)
-     apply (simp add: spec_def put_def put_state_def  get_state_def low_Env_def)
-   apply (intro seq_rule[of _ _ "(\<lambda>x y. high y - i y = high e - i e \<and> high e > i e)"])
-    apply (simp add: spec_def put_def put_state_def swap_def get_state_def xs_Env_def)
-   apply(intro allI; simp)
-   apply(intro get_rule; intro allI)
-   apply (intro seq_rule[of _ _ "(\<lambda>x y. Suc(high y - i y) = high e - i e)"])
-    apply (simp add: spec_def put_def put_state_def get_state_def i_Env_def)
-     apply linarith
-   apply(intro allI; simp)
-   apply(intro get_rule; intro allI)
-    apply (simp add: spec_def put_def put_state_def get_state_def low_Env_def)
+  apply(simp add: inc_lowbound_def)
+  apply(intro get_rule; intro allI; simp)
+  apply(intro conj_rule_right)
+  apply (intro seq_rule[of _ _ "(\<lambda>_ y. length (xs e) = length (xs y))"])
+  apply (simp add: spec_def put_def put_state_def swap_def get_state_def xs_Env_def)
+  apply(intro allI; simp)
+  apply(intro get_rule; intro allI)
+  apply (intro seq_rule[of _ _ "(\<lambda>_ y. length (xs e) = length (xs y))"])
+  apply (simp add: spec_def put_def put_state_def swap_def get_state_def i_Env_def)
+  apply(intro allI; simp)
+  apply(intro get_rule; intro allI)
+  apply (simp add: spec_def put_def put_state_def swap_def get_state_def low_Env_def)
+  apply (intro seq_rule[of _ _ "(\<lambda>_ y. high e = high y)"])
+  apply (simp add: spec_def put_def put_state_def swap_def get_state_def xs_Env_def)
+  apply(intro allI; simp)
+  apply(intro get_rule; intro allI)
+  apply (intro seq_rule[of _ _ "(\<lambda>_ y. high e = high y)"])
+  apply (simp add: spec_def put_def put_state_def swap_def get_state_def i_Env_def)
+  apply(intro allI; simp)
+  apply(intro get_rule; intro allI)
+  apply (simp add: spec_def put_def put_state_def swap_def get_state_def low_Env_def)
+  apply (intro seq_rule[of _ _ "(\<lambda>_ y. low e = low y)"])
+  apply (simp add: spec_def put_def put_state_def swap_def get_state_def xs_Env_def i_Env_def)
+  apply(intro allI; simp)
+  apply(intro get_rule; intro allI)
+  apply(intro seq_rule[of _ _ "(\<lambda>_ y. low e = low y)"])
+  apply (simp add: spec_def put_def put_state_def  get_state_def i_Env_def)
+  apply(intro allI; simp)
+  apply(intro get_rule; intro allI)
+  apply(simp add: spec_def put_def get_state_def put_state_def low_Env_def)
+  apply (intro seq_rule[of _ _ "(\<lambda>_ y. i y = i e)"])
+  apply (simp add: spec_def put_def put_state_def swap_def get_state_def xs_Env_def)
+  apply(intro allI; simp)
+  apply(intro get_rule; intro allI)
+  apply (intro seq_rule[of _ _ "(\<lambda>_ y. i y > i e)"])
+  apply (simp add: spec_def put_def put_state_def  get_state_def i_Env_def)
+  apply(intro allI; simp)
+  apply(intro get_rule; intro allI)
+  apply (simp add: spec_def put_def put_state_def  get_state_def low_Env_def)
+  apply (intro seq_rule[of _ _ "(\<lambda>_ y. i y < high y \<and> i y = i e \<and> high y = high e)"])
+  apply (simp add: spec_def put_def put_state_def swap_def get_state_def xs_Env_def)
+  apply(intro allI; simp)
+  apply(intro get_rule; intro allI)
+  apply (intro seq_rule[of _ _ "(\<lambda>_ y. high y - i y < high e - i e)"])
+  apply (simp add: spec_def put_def put_state_def  get_state_def i_Env_def)
+  apply (linarith)
+  apply(intro allI; simp)
+  apply(intro get_rule; intro allI)
+  apply (simp add: spec_def put_def put_state_def  get_state_def low_Env_def)
+  apply (intro seq_rule[of _ _ "(\<lambda>_ y. mset(xs e) = mset(xs y))"])
+  apply (simp add: spec_def put_def put_state_def swap_def get_state_def xs_Env_def)
+  apply (simp add: Multiset.mset_swap)
+  apply(intro allI; simp)
+  apply(intro get_rule; intro allI)
+  apply (intro seq_rule[of _ _ "(\<lambda>_ y. mset(xs e) = mset(xs y))"])
+  apply (simp add: spec_def put_def put_state_def get_state_def i_Env_def)
+  apply(intro allI; simp)
+  apply(intro get_rule; intro allI)
+  apply (simp add: spec_def put_def put_state_def  get_state_def low_Env_def)
+  apply (intro seq_rule[of _ _ "(\<lambda>x y. high y - i y = high e - i e \<and> high e > i e)"])
+  apply (simp add: spec_def put_def put_state_def swap_def get_state_def xs_Env_def)
+  apply(intro allI; simp)
+  apply(intro get_rule; intro allI)
+  apply (intro seq_rule[of _ _ "(\<lambda>x y. Suc(high y - i y) = high e - i e)"])
+  apply (simp add: spec_def put_def put_state_def get_state_def i_Env_def)
+  apply linarith
+  apply(intro allI; simp)
+  apply(intro get_rule; intro allI)
+  apply (simp add: spec_def put_def put_state_def get_state_def low_Env_def)
 
-    apply(simp add: dec_highbound_def)
-    apply(intro conj_rule_right)
-        apply (intro get_rule; intro allI; simp)
-        apply (intro seq_rule[of _ _ "(\<lambda>_ y. length (xs e) = length (xs y))"])
-         apply (simp add: spec_def put_def get_state_def put_state_def high_Env_def swap_def)
-        apply (rule allI; simp; intro get_rule; rule allI; simp)
-         apply (simp add: spec_def get_def put_def get_state_def put_state_def xs_Env_def swap_def)
-       apply (intro get_rule; intro allI; simp)
-          apply(intro seq_rule[of _ _ "(\<lambda>x y. high y < high e)"]) 
-        apply (simp add: spec_def get_def put_def get_state_def put_state_def high_Env_def)
-      apply (intro allI; simp)
-        apply (intro get_rule; intro allI; simp)
-         apply (simp add: spec_def get_def put_def get_state_def put_state_def xs_Env_def swap_def)
-      apply (intro get_rule; intro allI; simp)
-          apply(intro seq_rule[of _ _ "(\<lambda>x y. low e \<le> low y)"]) 
-        apply (simp add: spec_def get_def put_def get_state_def put_state_def high_Env_def)
-      apply (intro allI; simp)
-      apply (intro get_rule; intro allI; simp)
-         apply (simp add: spec_def get_def put_def get_state_def put_state_def xs_Env_def swap_def)
-      apply (intro get_rule; intro allI; simp)
-          apply(intro seq_rule[of _ _ "(\<lambda>x y. i e \<le> i y)"]) 
-        apply (simp add: spec_def get_def put_def get_state_def put_state_def high_Env_def)
-      apply (intro allI; simp)
-      apply (intro get_rule; intro allI; simp)
-       apply (simp add: spec_def get_def put_def get_state_def put_state_def xs_Env_def swap_def)
-      apply (intro get_rule; intro allI; simp)
-      apply(intro seq_rule[of _ _ "(\<lambda>x y. high y - i y < high e - i e)"]) 
-      apply (simp add: spec_def get_def put_def get_state_def put_state_def high_Env_def)
+  apply(simp add: dec_highbound_def)
+  apply(intro conj_rule_right)
+  apply (intro get_rule; intro allI; simp)
+  apply (intro seq_rule[of _ _ "(\<lambda>_ y. length (xs e) = length (xs y))"])
+  apply (simp add: spec_def put_def get_state_def put_state_def high_Env_def swap_def)
+  apply (rule allI; simp; intro get_rule; rule allI; simp)
+  apply (simp add: spec_def get_def put_def get_state_def put_state_def xs_Env_def swap_def)
+  apply (intro get_rule; intro allI; simp)
+  apply(intro seq_rule[of _ _ "(\<lambda>x y. high y < high e)"]) 
+  apply (simp add: spec_def get_def put_def get_state_def put_state_def high_Env_def)
+  apply (intro allI; simp)
+  apply (intro get_rule; intro allI; simp)
+  apply (simp add: spec_def get_def put_def get_state_def put_state_def xs_Env_def swap_def)
+  apply (intro get_rule; intro allI; simp)
+  apply(intro seq_rule[of _ _ "(\<lambda>x y. low e \<le> low y)"]) 
+  apply (simp add: spec_def get_def put_def get_state_def put_state_def high_Env_def)
+  apply (intro allI; simp)
+  apply (intro get_rule; intro allI; simp)
+  apply (simp add: spec_def get_def put_def get_state_def put_state_def xs_Env_def swap_def)
+  apply (intro get_rule; intro allI; simp)
+  apply(intro seq_rule[of _ _ "(\<lambda>x y. i e \<le> i y)"]) 
+  apply (simp add: spec_def get_def put_def get_state_def put_state_def high_Env_def)
+  apply (intro allI; simp)
+  apply (intro get_rule; intro allI; simp)
+  apply (simp add: spec_def get_def put_def get_state_def put_state_def xs_Env_def swap_def)
+  apply (intro get_rule; intro allI; simp)
+  apply(intro seq_rule[of _ _ "(\<lambda>x y. high y - i y < high e - i e)"]) 
+  apply (simp add: spec_def get_def put_def get_state_def put_state_def high_Env_def)
   apply(linarith)
-     apply(intro allI; simp)
-    apply (intro get_rule; intro allI; simp)
-    apply (simp add: spec_def get_def put_def get_state_def put_state_def xs_Env_def swap_def)
-    apply (intro get_rule; intro allI; simp)
-   apply (intro seq_rule[of _ _ "(\<lambda>_ y. mset(xs e) = mset(xs y))"])
-    apply (simp add: spec_def put_def put_state_def swap_def get_state_def high_Env_def)
-   apply(intro allI; simp)
-    apply(intro get_rule; intro allI; simp)
-    apply (simp add: spec_def get_def put_def get_state_def put_state_def xs_Env_def swap_def)
-    apply (simp add: Multiset.mset_swap)
-    apply(intro get_rule; intro allI; simp)
+  apply(intro allI; simp)
+  apply (intro get_rule; intro allI; simp)
+  apply (simp add: spec_def get_def put_def get_state_def put_state_def xs_Env_def swap_def)
+  apply (intro get_rule; intro allI; simp)
+  apply (intro seq_rule[of _ _ "(\<lambda>_ y. mset(xs e) = mset(xs y))"])
+  apply (simp add: spec_def put_def put_state_def get_state_def high_Env_def)
+  apply(intro allI; simp)
+  apply(intro get_rule; intro allI; simp)
+  apply (simp add: spec_def get_def put_def get_state_def put_state_def xs_Env_def swap_def)
+  apply (simp add: Multiset.mset_swap)
+  apply(intro get_rule; intro allI; simp)
 
-   apply (intro seq_rule[of _ _ "(\<lambda>x y. Suc(high y - i y) = high e - i e \<and> high e > i e)"])
-         apply (simp add: spec_def put_def put_state_def get_state_def high_Env_def)
-        apply linarith
-   apply(intro allI; simp)
-   apply(intro get_rule; intro allI; simp)
+  apply (intro seq_rule[of _ _ "(\<lambda>x y. Suc(high y - i y) = high e - i e \<and> high e > i e)"])
+  apply (simp add: spec_def put_def put_state_def get_state_def high_Env_def)
+  apply linarith
+  apply(intro allI; simp)
+  apply(intro get_rule; intro allI; simp)
   apply (simp add: spec_def put_def put_state_def get_state_def xs_Env_def)
-   apply(simp add: inc_index_def)
-    apply (intro get_rule; intro allI; simp)
-    apply (simp add: spec_def get_def put_def get_state_def put_state_def i_Env_def)
+  apply(simp add: inc_index_def)
+  apply (intro get_rule; intro allI; simp)
+  apply (simp add: spec_def get_def put_def get_state_def put_state_def i_Env_def)
   apply (simp add: diff_le_mono2)
   by (simp add: Suc_diff_Suc)
 
 subsection\<open>Invariants - Loop update action \<close>                                                       
-lemma loop_update_action_invariantRed: "spec loop_update_action_inv1_aux loop_update_action (GG loop_update_action_inv1)"
-   unfolding loop_update_action_inv1_aux_def loop_update_action_inv1_def dnfp_variables_invariants_def  loop_update_action_pre_def  GG_def low_invariant_is_0_Env_def
-  apply(simp add: loop_update_action_def)
-  apply (intro get_rule; intro allI; clarify)
+lemma loop_update_action_invariantRed: "spec loop_update_action_inv1 loop_update_action (GG dnfp_inv1)"
+   unfolding loop_update_action_inv1_def loop_update_action_inv1_def dnfp_variables_invariants_def dnfp_inv1_def  loop_update_action_pre_def  GG_def low_invariant_is_0_Env_def
+   apply(simp add: loop_update_action_def)
+   apply (intro get_rule; intro allI; clarify)
    apply (intro cond_rule)
-     apply(simp add: inc_lowbound_def)
-     apply (intro get_rule; intro allI; simp)
-  apply(intro seq_rule[of _ _ "(\<lambda>x e. i e < high e \<and>
+   apply(simp add: inc_lowbound_def)
+   apply (intro get_rule; intro allI; simp)
+   apply(intro seq_rule[of _ _ "(\<lambda>x e. i e < high e \<and>
                                 low e \<le> i e \<and>
                                 high e \<le> length (xs e) \<and> set (xs e) \<subseteq> {0, 1, 2} \<and> (\<forall>x\<le>low e. xs e ! x = 0))"])
-      apply (simp add: spec_def put_def put_state_def swap_def get_state_def xs_Env_def)
+   apply (simp add: spec_def put_def put_state_def swap_def get_state_def xs_Env_def)
    apply (smt le_antisym le_eq_less_or_eq le_trans length_list_update nth_list_update_eq nth_list_update_neq)
-  apply(intro allI; simp)
-  apply(intro get_rule; intro allI)
-  apply(intro seq_rule[of _ _ "(\<lambda>x e. i e \<le> high e \<and>
+   apply(intro allI; simp)
+   apply(intro get_rule; intro allI)
+   apply(intro seq_rule[of _ _ "(\<lambda>x e. i e \<le> high e \<and>
                low e < i e \<and>
                high e \<le> length (xs e) \<and> set (xs e) \<subseteq> {0, 1, 2} \<and> (\<forall>x\<le>low e. xs e ! x = 0))"])
-      apply (simp add: spec_def put_def put_state_def get_state_def i_Env_def)
-  apply(intro allI; simp)
-  apply(intro get_rule; intro allI)
-     apply (simp add: spec_def put_def put_state_def get_state_def low_Env_def)
-     apply(simp add: dec_highbound_def)
-     apply (intro get_rule; intro allI; simp)
-      apply(intro seq_rule[of _ _ "(\<lambda>_ e. i e \<le> high e \<and>
+   apply (simp add: spec_def put_def put_state_def get_state_def i_Env_def)
+   apply(intro allI; simp)
+   apply(intro get_rule; intro allI)
+   apply (simp add: spec_def put_def put_state_def get_state_def low_Env_def)
+   apply(simp add: dec_highbound_def)
+   apply (intro get_rule; intro allI; simp)
+   apply(intro seq_rule[of _ _ "(\<lambda>_ e. i e \<le> high e \<and>
                low e \<le> i e \<and>
                high e \<le> length (xs e) \<and> set (xs e) \<subseteq> {0, 1, 2} \<and> (\<forall>x<low e. xs e ! x = 0))"]) 
-       apply (simp add: spec_def get_def put_def get_state_def put_state_def high_Env_def)
-       apply(linarith)
-      apply(intro allI; simp)
-     apply (intro get_rule; intro allI; simp)
-      apply (simp add: spec_def get_def put_def get_state_def put_state_def xs_Env_def swap_def)
-     apply(simp add: inc_index_def)
-     apply (intro get_rule; intro allI; simp)
+   apply (simp add: spec_def get_def put_def get_state_def put_state_def high_Env_def)
+   apply(linarith)
+   apply(intro allI; simp)
+   apply (intro get_rule; intro allI; simp)
+   apply (simp add: spec_def get_def put_def get_state_def put_state_def xs_Env_def swap_def)
+   apply(simp add: inc_index_def)
+   apply (intro get_rule; intro allI; simp)
    by (simp add: spec_def get_def put_def get_state_def put_state_def i_Env_def)
 
-lemma loop_update_action_invariantWhite: "spec loop_update_action_inv2_aux loop_update_action (GG loop_update_action_inv2)"
-   unfolding loop_update_action_inv2_aux_def GG_def
-  apply(simp add: loop_update_action_def)
-  apply (intro get_rule; intro allI; clarify)
+ text\<open>The following proofs are mostly done using the already established lemmas of the definitions inside loop update action.\<close>
+lemma loop_update_action_invariantWhite: "spec loop_update_action_inv2 loop_update_action (GG dnfp_inv2)"
+   unfolding loop_update_action_inv2_def GG_def
+   apply(simp add: loop_update_action_def)
+   apply (intro get_rule; intro allI; clarify)
    apply (intro cond_rule; simp)
-    apply (smt GG_def case_prodD case_prodI2 inc_lowbound_inv2_aux_def inc_lowbound_inv2_def inc_lowbound_invariantWhite less_numeral_extra(1) loop_update_action_inv2_def spec_def)
-    apply (smt GG_def One_nat_def dec_highbound_inv2_aux_def dec_highbound_inv2_def dec_highbound_invariantWhite loop_update_action_inv2_def spec_def split_beta')
-   by (smt GG_def One_nat_def Suc_less_eq inc_index_inv2_aux_def inc_index_inv2_def inc_index_invariantWhite less_Suc_eq loop_update_action_inv2_def spec_def split_beta')
+   apply (smt GG_def case_prodD case_prodI2  inc_lowbound_inv2_def inc_lowbound_invariantWhite less_numeral_extra(1) loop_update_action_inv2_def spec_def)
+   apply (smt GG_def One_nat_def  dec_highbound_inv2_def dec_highbound_invariantWhite loop_update_action_inv2_def spec_def split_beta')
+   by (smt GG_def One_nat_def Suc_less_eq inc_index_inv2_def inc_index_invariantWhite less_Suc_eq loop_update_action_inv2_def spec_def split_beta')
    
-lemma loop_update_action_invariantBlue: "spec loop_update_action_inv3_aux loop_update_action (GG loop_update_action_inv3)"
-   unfolding loop_update_action_inv3_aux_def GG_def 
-  apply(simp add: loop_update_action_def)
-  apply (intro get_rule; intro allI; clarify)
+lemma loop_update_action_invariantBlue: "spec loop_update_action_inv3 loop_update_action (GG dnfp_inv3)"
+   unfolding loop_update_action_inv3_def GG_def 
+   apply(simp add: loop_update_action_def)
+   apply (intro get_rule; intro allI; clarify)
    apply (intro cond_rule;simp)
-     apply (smt GG_def case_prodD case_prodI2 inc_lowbound_inv3_aux_def inc_lowbound_inv3_def inc_lowbound_invariantBlue less_numeral_extra(1) loop_update_action_inv3_def spec_def)
-    apply (smt GG_def One_nat_def dec_highbound_inv3_aux_def dec_highbound_inv3_def dec_highbound_invariantBlue loop_update_action_inv3_def spec_def split_beta')
-   by (smt GG_def One_nat_def Suc_less_eq inc_index_inv3_aux_def inc_index_inv3_def inc_index_invariantBlue less_Suc_eq loop_update_action_inv3_def spec_def split_beta')
+   apply (smt GG_def case_prodD case_prodI2  inc_lowbound_inv3_def inc_lowbound_invariantBlue less_numeral_extra(1) loop_update_action_inv3_def spec_def)
+   apply (smt GG_def One_nat_def  dec_highbound_inv3_def dec_highbound_invariantBlue loop_update_action_inv3_def spec_def split_beta')
+   by (smt GG_def One_nat_def Suc_less_eq  inc_index_inv3_def inc_index_invariantBlue less_Suc_eq loop_update_action_inv3_def spec_def split_beta')
 
-lemma loop_update_action_invariants: "spec loop_update_action_inv_aux loop_update_action (GG loop_update_action_inv)"
-  unfolding loop_update_action_inv_aux_def GG_def loop_update_action_inv_def
-  by (smt GG_def case_prodD case_prodI2 loop_update_action_inv1_aux_def loop_update_action_inv2_aux_def loop_update_action_inv3_aux_def loop_update_action_invariantBlue loop_update_action_invariantRed loop_update_action_invariantWhite spec_def)
-
+lemma loop_update_action_invariants: "spec loop_update_action_inv loop_update_action (GG dnfp_inv)"
+  unfolding loop_update_action_inv_def GG_def loop_update_action_inv_def dnfp_inv_def
+  by (smt GG_def case_prodD case_prodI2 loop_update_action_inv1_def loop_update_action_inv2_def loop_update_action_inv3_def loop_update_action_invariantBlue loop_update_action_invariantRed loop_update_action_invariantWhite spec_def)
 end
